work on ImplFlushRootBucket

disk-betree/ImplFlushRootBucket.i.dfy
@@ -1,29 +1,30 @@
 include "ImplCache.i.dfy"
+include "ImplModelFlushRootBucket.i.dfy"
 
 module ImplFlushRootBucket { 
   import opened Impl
   import opened ImplIO
   import opened ImplCache
+  import ImplModelFlushRootBucket
+  import opened ImplState
 
   import opened Options
-  import opened MainDiskIOHandler
   import opened Maps
   import opened Sequences
   import opened Sets
 
   import opened BucketsLib
 
-  method {:fuel BC.GraphClosed,0} flushRootBucket(k: ImplConstants, s: ImplVariables, io: DiskIOHandler)
+  method {:fuel BC.GraphClosed,0} flushRootBucket(k: ImplConstants, s: ImplVariables)
   returns (s': ImplVariables)
-  requires io.initialized()
-  modifies io
-  requires IS.WFVars(s)
-  requires BBC.Inv(k, IS.IVars(s))
+  requires Inv(k, s)
   requires s.Ready?
   requires s.rootBucket != TTT.EmptyTree
-  ensures IS.WFVars(s')
-  ensures ImplADM.M.Next(Ik(k), old(IS.IVars(s)), IS.IVars(s'), UI.NoOp, io.diskOp())
+  ensures WVars(s')
+  ensures IVars(s') == ImplModelFlushRootBucket.flushRootBucket(Ic(k), old(IVars(s)))
   {
+    ImplModelFlushRootBucket.reveal_flushRootBucket();
+
     var oldroot := s.cache[BT.G.Root()];
 
     var rootBucketSeq := TTT.AsSeq(s.rootBucket);
@@ -35,7 +36,6 @@ module ImplFlushRootBucket {
         && (forall i | 0 <= i < |rootBucketSeq| :: |rootBucketSeq[i].1.value| < 0x1_000)))
     {
       s' := s;
-      assert noop(k, old(IS.IVars(s)), IS.IVars(s'));
       print "giving up; rootBucketSeq too big\n";
       return;
     }
@@ -48,29 +48,16 @@ module ImplFlushRootBucket {
       && (forall i | 0 <= i < |oldroot.buckets| :: |oldroot.buckets[i].keys| < 0x4000_0000_0000_0000)
     )) {
       s' := s;
-      assert noop(k, old(IS.IVars(s)), IS.IVars(s'));
       print "giving up; kmt/oldroot.buckets too big\n";
       return;
     }
 
-    forall i, key | 0 <= i < |oldroot.buckets| && key in KMTable.I(oldroot.buckets[i]) ensures Pivots.Route(oldroot.pivotTable, key) == i
-    {
-      //assert BT.NodeHasWFBucketAt(IS.INode(oldroot), i);
-    }
-
     var newbuckets := KMTable.Flush(kmt, oldroot.buckets, oldroot.pivotTable);
-    WFBucketListFlush(KMTable.I(kmt), KMTable.ISeq(oldroot.buckets), oldroot.pivotTable);
 
     var newroot := oldroot.(buckets := newbuckets);
 
     s' := s.(rootBucket := TTT.EmptyTree)
         .(cache := s.cache[BT.G.Root() := newroot]);
-
-    BucketListFlushParentEmpty(KMTable.ISeq(newbuckets), oldroot.pivotTable);
-    assert IS.INodeRoot(oldroot, s.rootBucket) == IS.INodeRoot(newroot, TTT.EmptyTree);
-    assert IS.ICache(s.cache, s.rootBucket) == IS.ICache(s'.cache, TTT.EmptyTree);
-
-    assert noop(k, old(IS.IVars(s)), IS.IVars(s'));
   }
 
 }
